src/tls/MasterSecret.fst
@@ -6,91 +6,92 @@ open TLSConstants
 open StreamAE
 open TLSInfo
 module AE = StreamAE
-module MM = MonotoneMap
+module DM = FStar.DependentMap
+module MM = FStar.Monotonic.DependentMap
 module MR = FStar.Monotonic.RRef
 module HH = FStar.HyperHeap
 module N = Nonce
 module I = IdNonce
 
 //We maintain ms_tab, a map from ids i, to w:StreamAE.writer i
-//such that, w's region is known to be a child region of the 
+//such that, w's region is known to be a child region of the
 //region associated with i's nonce
 let writer (i:AE.id) = w:AE.writer i{
-  N.registered (nonce_of_id i) (HH.parent w.region) /\ 
+  N.registered (nonce_of_id i) (HH.parent w.region) /\
   HH.disjoint (HH.parent w.region) tls_region /\
   MR.witnessed (MR.rid_exists w.region) /\
   is_epoch_rgn w.region /\
   is_epoch_rgn (HH.parent w.region)
-}  
+}
 
 // A partial map from i:id to w:writer i is region_injective
 // if it maps distinct ids to writers with distinct regions
-let region_injective (m:MM.map' AE.id writer) = 
-  forall i1 i2.{:pattern (MM.sel m i1); (MM.sel m i2)} 
-       i1=!=i2 ==> (match MM.sel m i1, MM.sel m i2 with
-			  | Some w1, Some w2 -> w1.region <> w2.region
-			  | _ -> True)
+let region_injective (m:MM.partial_dependent_map AE.id writer) =
+  forall i1 i2.{:pattern (DM.sel m i1); (DM.sel m i2)}
+       i1=!=i2 ==> (match DM.sel m i1, DM.sel m i2 with
+                          | Some w1, Some w2 -> w1.region <> w2.region
+                          | _ -> True)
 
-let ms_tab : MM.t tls_tables_region AE.id writer region_injective = 
-  MM.alloc #TLSConstants.tls_tables_region #AE.id #writer #region_injective
+let ms_tab : MM.t tls_tables_region AE.id writer region_injective =
+  MM.alloc ()
 
 //A region is fresh if no nonce is associated with it
-let fresh_in_ms_tab (r:rgn) (h:mem) = 
-  forall i. match MM.sel (MR.m_sel h ms_tab) i with 
+let fresh_in_ms_tab (r:rgn) (h:mem) =
+  forall i. match MM.sel (MR.m_sel h ms_tab) i with
        | Some w -> w.region <> r
        | None -> True
 
-private let id_rgns_witnessed (m:MM.map' AE.id writer) = 
+private let id_rgns_witnessed (m:MM.map AE.id writer) =
     forall (i:AE.id{Some? (MM.sel m i)}). MR.witnessed (MR.rid_exists ((Some?.v (MM.sel m i)).region))
 
 private let contains_id_rgns (h:mem) =
-    let m = MR.m_sel h ms_tab in 
+    let m = MR.m_sel h ms_tab in
     forall (i:AE.id{Some? (MM.sel m i)}). Map.contains h.h ((Some?.v (MM.sel m i)).region)
 
 
 (* private val all_ms_tab_regions_exists: unit -> ST unit //would be good to make such stateful lemmas STTot, once we have it; a bit loose for now *)
 (*   (requires (fun h0 -> True)) *)
 (*   (ensures (fun h0 _ h1 ->  *)
-(* 	      h0=h1 /\ *)
-(* 	      contains_id_rgns h1)) *)
-let all_ms_tab_regions_exists () = 
+(*            h0=h1 /\ *)
+(*            contains_id_rgns h1)) *)
+let all_ms_tab_regions_exists () =
   MR.m_recall ms_tab;
   let m0 = MR.m_read ms_tab in
-  let tok : squash (id_rgns_witnessed m0) = () in   
+  let tok : squash (id_rgns_witnessed m0) = () in
   MR.testify_forall tok
 
-let derive (r:rgn) (i:AE.id) 
+let derive (r:rgn) (i:AE.id)
   : ST (AE.writer i)
-       (requires (fun h -> 
-	   HH.disjoint r tls_region /\
-	   is_epoch_rgn r /\
-	   N.registered (nonce_of_id i) r))
+       (requires (fun h ->
+           HH.disjoint r tls_region /\
+           is_epoch_rgn r /\
+           N.registered (nonce_of_id i) r))
        (ensures (fun h0 w h1 ->
-	   let ms_tab_as_hsref = MR.as_hsref ms_tab in
-       	   HH.disjoint r tls_region 
-	   /\ is_epoch_rgn r
-	   /\ N.registered (nonce_of_id i) r
-	   /\ HH.parent w.region = r
-	   /\ is_epoch_rgn w.region
-	   /\ modifies (Set.singleton tls_tables_region) h0 h1 //modifies at most the tls_tables region
-	   /\ modifies_rref tls_tables_region (Set.singleton (Heap.addr_of (HH.as_ref ms_tab_as_hsref.ref))) h0.h h1.h //and within it, at most ms_tab
-	   /\ MR.witnessed (MR.rid_exists w.region) //and the writer's region is witnessed to exists also
-	   /\ MR.witnessed (MM.contains ms_tab i w) //and the writer is witnessed to be in ms_tab
-	   /\ (let old_ms = MR.m_sel h0 ms_tab in
-	      let new_ms = MR.m_sel h1 ms_tab in
- 	       old_ms == new_ms //either ms_tab didn't change at all
-	       \/ (MM.sel old_ms i == None
-		  /\ new_ms == MM.upd old_ms i w //or we just added w to it
-	   	  /\ (TLSInfo.authId i ==> MR.m_sel h1 (AE.ilog w.log) == Seq.createEmpty))))) //and it is a fresh log
+           let ms_tab_as_hsref = MR.as_hsref ms_tab in
+           HH.disjoint r tls_region
+           /\ is_epoch_rgn r
+           /\ N.registered (nonce_of_id i) r
+           /\ HH.parent w.region = r
+           /\ is_epoch_rgn w.region
+           /\ modifies (Set.singleton tls_tables_region) h0 h1 //modifies at most the tls_tables region
+           /\ modifies_rref tls_tables_region (Set.singleton (Heap.addr_of (HH.as_ref ms_tab_as_hsref.ref))) h0.h h1.h //and within it, at most ms_tab
+           /\ MR.witnessed (MR.rid_exists w.region) //and the writer's region is witnessed to exists also
+           /\ MR.witnessed (MM.contains ms_tab i w) //and the writer is witnessed to be in ms_tab
+           /\ (let old_ms = MR.m_sel h0 ms_tab in
+              let new_ms = MR.m_sel h1 ms_tab in
+               old_ms == new_ms //either ms_tab didn't change at all
+               \/ (MM.sel old_ms i == None
+                  /\ new_ms == MM.upd old_ms i w //or we just added w to it
+                  /\ (TLSInfo.authId i ==> MR.m_sel h1 (AE.ilog w.log) == Seq.createEmpty))))) //and it is a fresh log
   = MR.m_recall ms_tab;
     match MM.lookup ms_tab i with
-    | None -> 
+    | None ->
       all_ms_tab_regions_exists ();
-      let w = AE.gen r i in 
+      let w = AE.gen r i in
       let wr = MR.ex_rid_of_rid w.region in //witness that it always exists
       MM.extend ms_tab i w;
       w
-    | Some w -> 
+    | Some w ->
       N.testify (nonce_of_id i) r;   // n i -> r
-      N.testify (nonce_of_id i) (HH.parent w.region); //n i -> HH.parent w.region ==> r=w.region; 
+      N.testify (nonce_of_id i) (HH.parent w.region); //n i -> HH.parent w.region ==> r=w.region;
       w
