src/tls/Standalone.fst
@@ -2,11 +2,11 @@ module Standalone
 open FStar.Bytes
 open FStar.HyperStack.ST
 open FStar.Monotonic.RRef
-module MM = MonotoneMapNonDep
+module MM = FStar.Monotonic.DependentMap
 module HH = FStar.HyperHeap
 module MR = FStar.Monotonic.RRef
 assume val some_region : HH.rid
 type random = lbytes 32
-let injective (n:MM.map' random rid) = True
-let nonce_rid_table : MM.t some_region random MR.ex_rid injective =
+let injective (n:MM.partial_dependent_map random (fun _ -> rid)) = True
+let nonce_rid_table : MM.t some_region random (fun _ -> MR.ex_rid) injective =
     MM.alloc ()
